theories/Dijkstra/ItreeDijkstra.v
@@ -18,6 +18,7 @@ From ITree Require Import
      Events.MapDefault
      Events.State
      Events.StateFacts
+     Dijkstra.DijkstraMonadExamples
 .
 
 Import Monads.
@@ -37,11 +38,47 @@ Section PureItree.
 
   (* can interpretation deal with infinite taus*)
 
-  Definition _PureItreeSpec A := (A + unit -> Prop) -> Prop.
+  Definition _PureItreeSpec A := (itree Void A-> Prop) -> Prop.
 
-  Definition _PureItreeSpec' A := (itree Void A -> Prop) -> Prop.
+  Definition _retpi A (a : A) : _PureItreeSpec A := fun p => p (ret a).
 
-  Definition retp A (a : A) := fun (p : A + unit -> Prop) => (p (inl a)).
+  (*I will axiomatize into existence two functions on itrees and talk to steve about if they are 
+   feasible*)
+  
+
+  Definition monotonici A (w : _PureItreeSpec A) :=
+    forall (p p' : itree Void A -> Prop), (forall i', p i' -> p' i') -> w p -> w p'. 
+
+ (* is is_val a decidable prop   *)
+  Inductive is_val A (a : A) : itree Void A -> Prop :=
+    | base (t : itree Void A ) :  t = ret a ->  is_val A a t
+    | tau (t : itree Void A) : is_val A a (Tau t) .
+
+  Definition _bindpi A B (m : _PureItreeSpec A ) (f : A -> _PureItreeSpec B) : _PureItreeSpec B :=
+    fun (p : itree Void B -> Prop) => 
+      m (fun (i : itree Void A) => forall a, is_val A a i -> f a p).
+
+  Lemma bindpi_monot : forall A B (w : _PureItreeSpec A) (f : A -> _PureItreeSpec B), 
+      monotonici A w -> (forall a, monotonici B (f a)) -> monotonici B (_bindpi A B w f).
+  Proof.
+    unfold monotonici. intros. unfold _bindpi in *. intros.
+    remember (fun i : itree Void A => forall a : A, is_val A a i -> f a p) as fp.
+    remember (fun i : itree Void A => forall a : A, is_val A a i -> f a p') as fp'.
+    enough (forall i, fp i -> fp' i).
+    - apply H with (p := fp); auto.
+    - subst. intros. apply H0 with (p := p); auto.
+  Qed.
+
+  (* does this satisfy the monad laws? is it unique in some sense, if not what are the implications of
+   this choice*)
+  
+  (* maybe could parameterize bind on a predicate is_val A a itree -> Prop, and that predicate
+     determines how nonterminism is handled, that shouldn't be hard, my proof of monot
+     didn't seem to rely on the def of is_val, likely bad choices would break monad laws?
+     *)
+                       
+
+(* is this monotonic?   *)
 
 End PureItree.
 
@@ -51,6 +88,56 @@ Section StateItree.
   Definition StateItree A := itree (stateE S) A.
 
   Definition _StateItreeSpec A := (itree Void (A * S) -> Prop) -> S -> Prop.
+
+  Definition _interpStateSpec : (stateE S) ~> (_StateSpec S) :=
+    fun _ (ev : stateE S _) =>
+      match ev with
+        | Get _ => fun p s => p (s,s)
+        | Put _ s => fun p s' => p (tt,s) end.
+
+  Lemma monot_interpStateSpec : forall A ev, monotonic S (_interpStateSpec A ev).
+    Proof.
+      unfold monotonic. intros. cbv. destruct ev; auto.
+    Qed.
+
+  Definition monotonicis A (w : _StateItreeSpec A) := 
+    forall (p p' : itree Void (A * S) -> Prop ) s, (forall i s', p (ret (i,s')) -> p' (ret (i,s')))
+                                                                      -> w p s -> w p' s.
+
+  Definition _retis A (a : A) : _StateItreeSpec A :=
+    fun p s => p (ret (a,s)).
+
+  Lemma retis_monot : forall A a, monotonicis A (_retis A a).
+  Proof.
+    unfold monotonicis. intros. unfold _retis in *. auto.
+  Qed.
+(* bind I think needs some coinduction, I'll leave it out for now
+  Definition _bindis A B (m : _StateItreeSpec A) (f : A -> _StateItreeSpec B) :=
+    fun p s => m (fun '(i,s') =>  ) s
+
+    if i = tau ^ ω then p (i,s') since i has either type _StateItreeSpec A or _StateItreeSpec B
+    else i = tau ^* (Ret a) then p (ret (a,s'))
+
+    problem is the first case doesn't terminate, need more info on coinduction from Steve maybe?
+*)
+
+
+
+  Definition StateItreeSpec A := {w : _StateItreeSpec A | monotonicis _ w}.
+
+  Definition interpStateSpecCore : forall A, (stateE S A) -> (itree Void (StateSpec S A)) :=
+    fun A ev => 
+    ret (exist _ (_interpStateSpec A ev) (monot_interpStateSpec A ev)).
+
+  Definition StateSpecT (M : Type -> Type) (A : Type) := (M (A * S)%type -> Prop) -> S -> Prop.
+
+(*
+  Global Instance StateSpecIter : Monad
+
+  Definition interpStateSpec (A : Type) (t : itree (stateE S) A) : 
+    StateSpecT  (itree Void) A := interp interpStateSpecCore t.
+
+  *)
 (*
   Definition _retsis A (a: A) : _StateItreeSpec A := fun p s => p (Itree.ret _ (a,s)).
 
